Validator/StateSetFormalism/Mods.lean
@@ -1,63 +1,15 @@
 import Validator.StateSetFormalism.Formula
 
 namespace Validator
-
 open Formula
-
--- TODO : clean up
 
 structure MODS n where
   vars : VarSet' n
   mods : List (PartialModel vars)
   deriving DecidableEq, Repr
-  -- No duplicates?
 
 namespace Formula.PartialModel
-/-
-def toStates {n} {V : VarSet' (2 * n)} (M : PartialModel V) : States n :=
-  M.models.image Model.unprimedState
 
-lemma mem_toStates {n} {V : VarSet' (2 * n)} {M : PartialModel V} {s : State n} :
-  s ∈ M.toStates ↔ ∀ i : Fin V.val.length, Even V.val[i] → (M[i] ↔ ⟨V.val[i] / 2, by omega⟩ ∈ s) :=
-  by
-    simp [toStates, Model.unprimedState, Fin.toUnprimed]
-    constructor
-    · rintro ⟨M', hM', rfl⟩ i h2
-      simp [PartialModel.models] at hM'
-      specialize hM' i
-      simp_all [Fin.even_iff_of_even, Nat.two_mul_div_two_of_even]
-    · intro h1
-      let M' : Model (2 * n) := fun ⟨i, hi⟩ ↦
-        match V.val.finIdxOf? ⟨i,hi⟩ with
-          | none => ⟨i / 2, by omega⟩ ∈ s
-          | some j => M[j]
-      have hM' : M' ∈ M.models := by
-        simp [M', models]
-        rintro ⟨j, hj⟩
-        specialize h1 ⟨j, hj⟩
-        split
-        case h_1 h =>
-          grind
-        case h_2 _ j' h2  =>
-          rcases j' with ⟨j', hj'⟩
-          obtain ⟨rfl⟩ : j = j' := by
-            have h3 := List.Sorted.nodup V.prop
-            rw [← List.Nodup.getElem_inj_iff h3 (hi := hj) (hj := hj')]
-            simp at h2 ⊢
-            simp_all only
-          rfl
-      use M', hM'
-      ext i
-      simp [M']
-      split
-      case h_1 => simp
-      case h_2 _ j h2 =>
-        simp at h2
-        have h3 : Even V.val[j] := by
-          simp [Fin.even_iff_of_even, h2.1]
-        specialize h1 j h3
-        simp_all
--/
 lemma models_nonempty {n} {V : VarSet' n} (M : PartialModel V) : Nonempty M.models :=
   by
     constructor
@@ -101,22 +53,24 @@ lemma mem_models_to_mem_literal_models
     rw [← h1, ← h2]
     exact h3 i
 
-end Formula.PartialModel
+end PartialModel
 
-namespace MODS
+namespace Clause
 
-/-
-def toStates {n} (φ : MODS n) : States n :=
-  φ.models.toList.biUnion Model.toStates
+private def isTrivial_aux {n} (acc : Vector (Bool × Bool) n) : Clause n → Vector (Bool × Bool) n
+| [] => acc
+| (x, true) :: ls => isTrivial_aux (acc.set x (true, acc[x].2)) ls
+| (x, false) :: ls => isTrivial_aux (acc.set x (acc[x].1, true)) ls
 
-@[simp]
-lemma mem_toStates {n} {φ : MODS n} {s} : s ∈ φ.toStates ↔ ∃ M ∈ φ.models, s ∈ M.toStates :=
+def isTrivial {n} (γ : Clause n) : Bool :=
+  (isTrivial_aux (Vector.replicate n (false, false)) γ).contains (true, true)
+
+lemma isTrivial_iff {n} {γ : Clause n} : isTrivial γ ↔ ∃ x, (x, true) ∈ γ ∧ (x, false) ∈ γ :=
   by
-    simp [toStates]
+    sorry
 
-#eval [∅, {0}, {1}, {0,1}].map
-  (fun x ↦ decide (x ∈ MODS.toStates ⟨(⟨#[0], by simp⟩ : OrderedVars (2 + 2)), #[#v[true]]⟩))
--/
+end Formula.Clause
+namespace MODS
 
 def models {n} (φ : MODS n) : Models n :=
   { M | ∃ M' ∈ φ.mods, M ∈ PartialModel.models M' }
@@ -136,16 +90,6 @@ instance {n} : Formula n (MODS n) where
     simp [models, PartialModel.models]
     grind
 
-/-
-  ofModel {V} M := MODS.mk V #[M]
-
-  ofModel_correct :=
-    by
-      intro V M
-      ext s
-      simp
--/
-
 instance {n} : Top n (MODS n) where
 
   top := sorry
@@ -158,24 +102,6 @@ instance {n} : Bot n (MODS n) where
 
   bot_correct := sorry
 
-/- TODO : remove
-instance {n} : ModelTesting n (MODS n) where
-
-  isModel φ M := φ.mods.contains M
-
-  isModel_correct :=
-    by
-      intro φ mod
-      simp [Formula.models]
-      constructor
-      · tauto
-      · intro h1
-        obtain ⟨M, h2⟩ := mod.models_nonempty
-        obtain ⟨M', hM', h3⟩ := h1 h2
-        rw [PartialModel.disjoint h2 h3]
-        exact hM'
--/
-
 instance {n} : ClausalEntailment n (MODS n) where
 
   -- This only seems to work is all variables of γ are in φ.vars
@@ -185,43 +111,35 @@ instance {n} : ClausalEntailment n (MODS n) where
   entails_correct :=
     by
       intro φ γ
-      sorry
-      /-
-      simp [Formalism.models, Finset.subset_iff, Clause.isTrivial_iff, -Bool.exists_bool, -Bool.forall_bool]
+      simp [Formula.models, Set.subset_def, Clause.isTrivial_iff, -Bool.exists_bool]
       constructor
-      · rintro h s M hM hs
-        obtain ⟨i, hi, rfl⟩ := Array.getElem_of_mem hM
+      · intro h M M' hM' hM
         rcases h with h | ⟨x, h⟩
-        · specialize h i hi
+        · obtain ⟨i, hi, rfl⟩ := List.getElem_of_mem hM'
+          specialize h φ.mods[i] hM'
           rcases h with ⟨var, b, h1, h2⟩
           use var, b, h1
-          exact Model.mem_model_to_mem_literal h2 hs
-        · if h : x ∈ s then
+          exact PartialModel.mem_models_to_mem_literal_models h2 hM
+        · if h : M x then
             use x, true
-            simp_all [Literal.mem_toFinset]
-            sorry
+            simp_all [Literal.mem_models]
           else
             use x, false
-            simp_all [Literal.mem_toFinset]
-            sorry
+            simp_all [Literal.mem_models]
       · intro h
         if h' : ∃ x, (x, true) ∈ γ ∧ (x, false) ∈ γ then
           exact Or.inr h'
         else
           apply Or.inl
-          intro i hi
-          obtain ⟨s, hs⟩ := Model.nonempty φ.models[i]
-          rcases h φ.models[i] (by simp) hs with ⟨var, b, h1, h2⟩
+          intro M' hM'
+          obtain ⟨M, hM⟩ := M'.models_nonempty
+          rcases h M M' hM' hM with ⟨var, b, h1, h2⟩
           use var, b, h1
-          simp [Model.mem_iff] at hs
-          simp_all [Literal.mem_toFinset, Model.contains_literal_iff]
-
+          simp_all [Literal.mem_models, PartialModel.contains_literal_iff]
           by_contra h3
           simp at h3
           obtain ⟨j, hj, h3⟩ := List.getElem_of_mem h1
-
-          sorry-/
-
+          sorry
 
 instance {n} : BoundedConjuction n (MODS n) where
 
@@ -237,9 +155,10 @@ instance {n} : SententialEntailment n (MODS n) where
 
 instance {n} : OfPartialModel n (MODS n) where
 
-  ofPartialModel := sorry
+  ofPartialModel V M := ⟨V, [M]⟩
 
-  ofPartialModel_correct := sorry
+  ofPartialModel_correct := by
+    simp [Formula.models, models, Formula.vars]
 
 instance {n} : Renaming n (MODS n) where
 
@@ -253,136 +172,4 @@ instance {n} : ToCNF n (MODS n) where
 
   toCNF_correct := sorry
 
-/-
-def models {n} (pt : STRIPS n) (φ : ConstantStateSet) : Models (2 * n) :=
-  (φ.partialModel pt).snd.models
--/
-/-
-  constant
-  | .empty => ⟨mkEmpty n, VarSet'.isUnprimed_unprimedVars⟩
-  | .init => ⟨mkInit pt, VarSet'.isUnprimed_unprimedVars⟩
-  | .goal => ⟨mkGoal pt, by
-    simp [mkGoal, Formula.vars]
-    exact VarSet'.isUnprimed_toUnprimed⟩
-
-/-
-  constant_eq
-  | .empty => by
-    simp [mkEmpty, Formula.models, models, List.biUnion]
-  | .init => by
-    ext s
-    simp [mkInit, Formula.models]
-    constructor
-    · rintro ⟨M, ⟨M', h1, h2⟩, rfl⟩
-      simp_all [unprimedVars]
-      rw [Vector.toArray_inj] at h1
-      sorry
-    · obtain ⟨M, hM⟩ := Model.exists_model_of_state s
-      sorry
-    rw [Vector.toArray_inj]
-
-    sorry
-  | .goal => sorry
--/
-  constant_eq
-  | .empty => by
-    simp [mkEmpty, ConstantStateSet.toStates]
-  | .init => by
-    ext s
-    simp [mkInit, PartialModel.mem_toStates, VarSet'.unprimedVars, Fin.toUnprimed]
-    constructor
-    · rintro h ⟨i, hi⟩
-      specialize h ⟨i, by simp [hi]⟩ (by simp [Fin.even_iff_of_even])
-      simp_all
-    · intro h
-      rintro ⟨i, hi⟩
-      simp [h ⟨i, by simp_all only [List.length_ofFn]⟩]
-  | .goal => by
-    ext s
-    simp [mkGoal, PartialModel.mem_toStates, VarSet'.toUnprimed, Fin.toUnprimed]
-    constructor
-    · rintro h i hi
-      obtain ⟨j, hj, h1⟩ := List.getElem_of_mem hi
-      specialize h ⟨j, by simp [hj]⟩ (by simp [Fin.even_iff_of_even])
-      simp_all
-    · intro h
-      rintro ⟨i, hi⟩ h1
-      apply h
-      simp
--/
-end MODS
-
-/-
-namespace old
-
-abbrev Model k := BitVec k
-
-structure Mods n where
-  vars : VarSet' n
-  models : Array (Model vars.size)
-  -- No duplicates?
-
-def Mods.toFinset {n} (φ : Mods n) : States n :=
-  Array.foldl (fun S M ↦ S ∪ Model.toFinset M) ∅ φ.models where
-
-  toModel (s : State n) : Model φ.vars.size :=
-    BitVec.ofFnLE (fun i ↦ decide (φ.vars[i] ∈ s))
-
-  Model.toFinset : Model φ.vars.size → States n
-  | M => {s ∈ (Fintype.elems : States n) | toModel s = M}
-
-#eval [∅, {0}, {1}, {0,1}].map (fun x ↦ decide (x ∈ Mods.toFinset ⟨(#[1] : VarSet' 2), #[]⟩))
-
-instance {n} : Formalism n (Mods n) where
-
-  OrderedVars φ := φ.vars
-
-  toFinset := Mods.toFinset
-
-instance {n} : BoundedConjuction n (Mods n) where
-
-  and φ ψ := sorry
-
-  and_correct := sorry
-
-instance {n} : SententialEntailment' n (Mods n) where
-
-  entails φ ψ h := sorry
-
-  entails_correct := sorry
-
-end old
--/
-/-
-CE -> is_entailed
-bool ModsStateSet::is_entailed(const VariableOrder &OrderedVars,
-                               const std::vector<bool> &clause) const {
-    std::vector<std::pair<int,int>> possible_checks;
-    for (size_t i = 0; i < OrderedVars.size(); ++i) {
-        for (size_t j = 0; j < formula.get_variable_order().size(); ++j) {
-            if (OrderedVars[i] == formula.get_variable_order()[j]) {
-                possible_checks.push_back({i,j});
-                break;
-            }
-        }
-    }
-    auto it = formula.get_cbegin();
-    while (it != formula.get_cend()) {
-        const Model &model = *it;
-        bool covered = false;
-        for (std::pair<int,int> check : possible_checks) {
-            if (model[check.second] == clause[check.first]) {
-                covered = true;
-                break;
-            }
-        }
-        if (!covered) {
-            return false;
-        }
-        it++;
-    }
-    return true;
-}
--/
-
-end Validator
+end Validator.MODS
